src3.0/Transforms/sas_msim.v
@@ -4,8 +4,10 @@ Require Import Coqlib.
 Require Import Integers.
 Require Import AST.
 Require Import Znumtheory.
-Require Import vellvm_tactics.
 Require Import memory_sim.
+Require Import vellvm.
+Require Import promotable_props.
+Require Import genericvalues_inject.
 
 Module SASmsim.
 
@@ -22,7 +24,14 @@ Module SASmsim.
 
 Export Mem.
 
-Record mem_inj (f: meminj) (b:block) (lo hi:Z) (m1 m2: mem) : Prop :=
+Definition notin_ignores (ignores:list (Values.block*Z*Z)) (b1:Values.block) 
+  (ofs:Z) : Prop :=
+List.Forall (fun ignore =>
+             let '(b,lo,hi) := ignore in
+             b1 <> b \/ (b1 = b /\ (ofs < lo \/ ofs >= hi))) ignores.
+
+Record mem_inj (f: meminj) (ignores:list (Values.block*Z*Z)) (m1 m2: mem) 
+  : Prop :=
   mk_mem_inj {
     mi_access:
       forall b1 b2 delta chunk ofs p,
@@ -33,7 +42,7 @@ Record mem_inj (f: meminj) (b:block) (lo hi:Z) (m1 m2: mem) : Prop :=
       forall b1 ofs b2 delta,
       f b1 = Some(b2, delta) ->
       perm m1 b1 ofs Nonempty ->
-      b1 <> b \/ (b1 = b /\ (ofs < lo \/ ofs >= hi)) ->
+      notin_ignores ignores b1 ofs ->
       MoreMem.memval_inject f (m1.(mem_contents) b1 ofs) 
         (m2.(mem_contents) b2 (ofs + delta))
   }.
@@ -41,8 +50,8 @@ Record mem_inj (f: meminj) (b:block) (lo hi:Z) (m1 m2: mem) : Prop :=
 (** Preservation of permissions *)
 
 Lemma perm_inj:
-  forall b lo hi f m1 m2 b1 ofs p b2 delta,
-  mem_inj f b lo hi m1 m2 ->
+  forall igns f m1 m2 b1 ofs p b2 delta,
+  mem_inj f igns m1 m2 ->
   perm m1 b1 ofs p ->
   f b1 = Some(b2, delta) ->
   perm m2 b2 (ofs + delta) p.
@@ -57,13 +66,56 @@ Qed.
 
 (** Preservation of loads. *)
 
+Definition notin_ignores_with_size (ignores:list (Values.block*Z*Z)) 
+  (b1:Values.block) (ofs:Z) (size:Z) : Prop :=
+List.Forall (fun ignore =>
+             let '(b,lo,hi) := ignore in
+             b1 <> b \/ (b1 = b /\ (ofs + size <= lo \/ ofs >= hi))) ignores.
+
+Lemma notin_ignores_with_size__notin_ignores: forall b ofs size (Hge: size > 0) 
+  igns, 
+  notin_ignores_with_size igns b ofs size ->
+  notin_ignores igns b ofs.
+Proof.
+  unfold notin_ignores_with_size, notin_ignores.
+  induction igns as [|[[]]]; simpl; intros; auto.
+    inv H.
+    constructor; auto.
+    destruct H2 as [H2 | [H6 [H4 | H4]]]; subst; auto.
+      right. split; auto. omega. 
+Qed.
+
+Lemma notin_ignores_with_size_delta: forall b ofs delta size igns
+  (J:delta>=0),
+  notin_ignores_with_size igns b ofs (delta+size) ->
+  notin_ignores_with_size igns b (ofs+delta) size.
+Proof.
+  unfold notin_ignores_with_size.
+  intros.
+  induction H; auto.
+    destruct x as [[b1 lo1] hi1].
+    constructor; auto.
+    destruct H as [H2 | [H6 [H4 | H4]]]; subst; try solve 
+      [auto | right; split; auto; omega]. 
+Qed.
+
+Lemma notin_ignores_with_size_inc: forall b ofs size igns, 
+  notin_ignores_with_size igns b ofs (Zsucc size) ->
+  notin_ignores_with_size igns b (ofs+1) size.
+Proof.
+  intros.
+  apply notin_ignores_with_size_delta; auto.
+    omega.
+    replace (1+size) with (Zsucc size) by omega. auto.
+Qed.
+
 Lemma getN_inj:
-  forall b lo hi f m1 m2 b1 b2 delta,
-  mem_inj f b lo hi m1 m2 ->
+  forall igns f m1 m2 b1 b2 delta,
+  mem_inj f igns m1 m2 ->
   f b1 = Some(b2, delta) ->
   forall n ofs,
   range_perm m1 b1 ofs (ofs + Z_of_nat n) Readable ->
-  b1 <> b \/ (b1 = b /\ (ofs + Z_of_nat n <= lo \/ ofs >= hi)) ->
+  notin_ignores_with_size igns b1 ofs (Z_of_nat n) ->
   list_forall2 (MoreMem.memval_inject f) 
                (getN n ofs (m1.(mem_contents) b1))
                (getN n (ofs + delta) (m2.(mem_contents) b2)).
@@ -77,27 +129,23 @@ Proof.
         apply perm_implies with Readable.
           apply H1. omega. 
           constructor. 
-        destruct H2 as [H2 | [H2 [H3 | H4]]]; subst; auto.
-        right. 
-        assert (J:=@Z_of_S_gt_O n).
-        split; try solve [auto | omega].
+        eapply notin_ignores_with_size__notin_ignores; eauto.
+        assert (J:=@Z_of_S_gt_O n). omega.
 
       replace (ofs + delta + 1) with ((ofs + 1) + delta) by omega.
       apply IHn. 
         red; intros; apply H1; omega. 
-
-        destruct H2 as [H2 | [H2 [H3 | H4]]]; subst; try solve 
-          [auto | right; split; try solve [auto | omega]].
+        apply notin_ignores_with_size_inc; auto.
 Qed.
 
 Lemma load_inj:
-  forall b lo hi f m1 m2 chunk b1 ofs b2 delta v1,
+  forall igns f m1 m2 chunk b1 ofs b2 delta v1,
   MoreMem.meminj_no_overlap f ->
   MoreMem.meminj_zero_delta f ->
-  mem_inj f b lo hi m1 m2 ->
+  mem_inj f igns m1 m2 ->
   load chunk m1 b1 ofs = Some v1 ->
   f b1 = Some (b2, delta) ->
-  b1 <> b \/ (b1 = b /\ (ofs + size_chunk chunk <= lo \/ ofs >= hi)) ->
+  notin_ignores_with_size igns b1 ofs (size_chunk chunk) ->
   exists v2, 
     load chunk m2 b2 (ofs + delta) = Some v2 /\ MoreMem.val_inject f v1 v2.
 Proof.
@@ -114,6 +162,23 @@ Local Transparent load.
     eapply getN_inj; eauto. 
       rewrite <- size_chunk_conv. exploit load_valid_access; eauto. intros [A B]. auto.
       rewrite <- size_chunk_conv. auto.
+Qed.
+
+Lemma load_inj2:
+  forall igns f m1 m2 chunk b1 ofs b2 delta v1 v2,
+  MoreMem.meminj_no_overlap f ->
+  MoreMem.meminj_zero_delta f ->
+  mem_inj f igns m1 m2 ->
+  load chunk m1 b1 ofs = Some v1 ->
+  f b1 = Some (b2, delta) ->
+  notin_ignores_with_size igns b1 ofs (size_chunk chunk) ->
+  load chunk m2 b2 (ofs + delta) = Some v2 ->
+  MoreMem.val_inject f v1 v2.
+Proof.
+  intros.
+  eapply load_inj in H2; eauto.
+  destruct H2 as [v2' [H2 H6]].
+  uniq_result. auto.
 Qed.
 
 (** Preservation of stores. *)
@@ -155,25 +220,16 @@ Proof.
   auto.
 Qed.
 
-(* go to Coqlib *)
-Lemma list_forall2_length_eq:
-  forall (A B: Type) (P1: A -> B -> Prop) (l1: list A) (l2: list B),
-  list_forall2 P1 l1 l2 -> length l1 = length l2.
-Proof.
-  induction 1; intros; auto.
-    simpl. congruence.
-Qed.
-
 Lemma store_mapped_inj:
-  forall b lo hi f chunk m1 b1 ofs v1 n1 m2 b2 delta v2,
-  mem_inj f b lo hi m1 m2 ->
+  forall igns f chunk m1 b1 ofs v1 n1 m2 b2 delta v2,
+  mem_inj f igns m1 m2 ->
   store chunk m1 b1 ofs v1 = Some n1 ->
   MoreMem.meminj_no_overlap f ->
   f b1 = Some (b2, delta) ->
   MoreMem.val_inject f v1 v2 ->
   exists n2,
     store chunk m2 b2 (ofs + delta) v2 = Some n2
-    /\ mem_inj f b lo hi n1 n2.
+    /\ mem_inj f igns n1 n2.
 Proof.
   intros. inversion H. 
   assert (valid_access m2 chunk b2 (ofs + delta) Writable).
@@ -218,16 +274,145 @@ Proof.
   eauto.
 Qed.
 
-Lemma store_mapped_inj_inside:
-  forall f chunk m1 b1 ofs v1 n1 m2 b2 delta v2,
-  mem_inj f b1 ofs (ofs+size_chunk chunk) m1 m2 ->
+Lemma store_mapped_inj2:
+  forall igns f chunk m1 b1 ofs v1 n1 m2 b2 delta v2 n2,
+  mem_inj f igns m1 m2 ->
   store chunk m1 b1 ofs v1 = Some n1 ->
   MoreMem.meminj_no_overlap f ->
   f b1 = Some (b2, delta) ->
   MoreMem.val_inject f v1 v2 ->
-  exists n2,
-    store chunk m2 b2 (ofs + delta) v2 = Some n2
-    /\ MoreMem.mem_inj f n1 n2.
+  store chunk m2 b2 (ofs + delta) v2 = Some n2 ->
+  mem_inj f igns n1 n2.
+Proof.
+  intros.
+  eapply store_mapped_inj in H0; eauto.
+  destruct H0 as [n2' [J1 J2]].
+  uniq_result. auto.
+Qed.
+
+Lemma store_unmapped_inj:
+  forall igns f chunk m1 b1 ofs v1 n1 m2,
+  mem_inj f igns m1 m2 ->
+  store chunk m1 b1 ofs v1 = Some n1 ->
+  f b1 = None ->
+  mem_inj f igns n1 m2.
+Proof.
+  intros. inversion H.
+  constructor.
+(* access *)
+  eauto with mem.
+(* mem_contents *)
+  intros. 
+  rewrite (store_mem_contents _ _ _ _ _ _ H0).
+  rewrite update_o. eauto with mem. 
+  congruence.
+Qed.
+
+Lemma store_outside_inj:
+  forall igns f m1 m2 chunk b ofs v m2',
+  mem_inj f igns m1 m2 ->
+  (forall b' delta ofs',
+    f b' = Some(b, delta) ->
+    perm m1 b' ofs' Nonempty ->
+    ofs' + delta < ofs \/ ofs' + delta >= ofs + size_chunk chunk) ->
+  store chunk m2 b ofs v = Some m2' ->
+  mem_inj f igns m1 m2'.
+Proof.
+  intros. inversion H. constructor.
+(* access *)
+  eauto with mem.
+(* mem_contents *)
+  intros. 
+  rewrite (store_mem_contents _ _ _ _ _ _ H1).
+  unfold update. destruct (zeq b2 b). subst b2.
+  rewrite setN_outside. auto. 
+  rewrite encode_val_length. rewrite <- size_chunk_conv. 
+  eapply H0; eauto. 
+  eauto with mem.
+Qed.
+
+Definition in_ignores_with_size (ignores:list (Values.block*Z*Z)) 
+  (b1:Values.block) (ofs:Z) (size:Z) : Prop :=
+exists b, exists lo, exists hi,
+  In (b,lo,hi) ignores /\ b1 = b /\ ofs + size <= hi /\ ofs >= lo.
+
+Lemma in_ignores_with_size__notin_ignores__inv: forall b ofs1 ofs2 size igns
+  (Hnzero: size>=0),
+  in_ignores_with_size igns b ofs1 size ->
+  notin_ignores igns b ofs2 ->
+  ofs2 < ofs1 \/ ofs2 >= ofs1 + size.
+Proof.
+  unfold in_ignores_with_size, notin_ignores.
+  intros.
+  destruct H as [b0 [lo0 [hi0 [H [J1 [J2 J3]]]]]]; subst.
+  induction igns as [|[[]]]; simpl; intros.
+    inv H.
+
+    inv H0.
+    simpl in H.
+    destruct H as [H | H]; eauto.
+    inv H.
+    destruct H3 as [H3 | [H3 [H5 | H5]]]; subst; try congruence; omega.
+Qed.
+
+Lemma store_inside_inj_left:
+  forall igns f m1 m2 chunk b ofs v m1',
+  mem_inj f igns m1 m2 ->
+  in_ignores_with_size igns b ofs (size_chunk chunk) ->
+  store chunk m1 b ofs v = Some m1' ->
+  mem_inj f igns m1' m2.
+Proof.
+  intros. inversion H. constructor.
+(* access *)
+  eauto with mem.
+(* mem_contents *)
+  intros. 
+  assert (perm m1 b1 ofs0 Nonempty) as Jp. 
+    eapply perm_store_2; eauto.
+  eapply mi_memval0 in Jp; eauto.
+  rewrite (store_mem_contents _ _ _ _ _ _ H1).
+  unfold update. 
+  destruct (zeq b1 b); subst; auto.
+    rewrite setN_outside; auto.
+      rewrite encode_val_length. rewrite <- size_chunk_conv.
+      eapply in_ignores_with_size__notin_ignores__inv; eauto.
+        assert (J:=@size_chunk_pos chunk). omega.
+Qed.
+
+Lemma store_inside_inj_left_inc:
+  forall igns f m1 m2 chunk b ofs lo hi v m1',
+  mem_inj f igns m1 m2 ->
+  lo <= ofs /\ ofs + (size_chunk chunk) <= hi ->
+  store chunk m1 b ofs v = Some m1' ->
+  mem_inj f ((b,lo,hi)::igns) m1' m2.
+Proof.
+  intros. inversion H. constructor.
+(* access *)
+  eauto with mem.
+(* mem_contents *)
+  intros. 
+  assert (perm m1 b1 ofs0 Nonempty) as Jp. 
+    eapply perm_store_2; eauto.
+  inv H4.
+  eapply mi_memval0 in Jp; eauto.
+  rewrite (store_mem_contents _ _ _ _ _ _ H1).
+  unfold update. 
+  destruct (zeq b1 b); subst; auto.
+    rewrite setN_outside; auto.
+      rewrite encode_val_length. rewrite <- size_chunk_conv.
+      destruct H7 as [H7 | [? [J | J]]]; try congruence; omega.
+Qed.
+
+Lemma store_inside_inj2':
+  forall igns f m1 m2 chunk b1 b2 ofs v1 v2 n1 delta hi,
+  mem_inj f ((b1,ofs,hi)::igns) m1 m2 ->
+  store chunk m1 b1 ofs v1 = Some n1 ->
+  MoreMem.meminj_no_overlap f ->
+  f b1 = Some (b2, delta) ->
+  MoreMem.val_inject f v1 v2 ->
+  exists n2, 
+    store chunk m2 b2 (ofs+delta) v2 = Some n2 /\
+    mem_inj f ((b1,ofs + (size_chunk chunk),hi)::igns) n1 n2.
 Proof.
   intros. inversion H. 
   assert (valid_access m2 chunk b2 (ofs + delta) Writable).
@@ -246,7 +431,7 @@ Proof.
   rewrite (store_mem_contents _ _ _ _ _ _ H0).
   rewrite (store_mem_contents _ _ _ _ _ _ STORE).
   unfold update. 
-  destruct (zeq b0 b1). subst b0.
+  destruct (zeq b0 b1); subst.
   (* block = b1, block = b2 *)
   assert (b3 = b2) by congruence. subst b3.
   assert (delta0 = delta) by congruence. subst delta0.
@@ -256,54 +441,66 @@ Proof.
     eapply list_forall2_length_eq; eauto.
   destruct (Z_gt_dec ofs ofs0).
     apply setN_inj_outside; auto.
-    eapply mi_memval0 in H7; eauto.
-      right. split; auto. omega.
+    assert (notin_ignores ((b1, ofs, hi) :: igns) b1 ofs0) 
+      as Higns.
+      unfold notin_ignores.
+      inv H7.
+      constructor; auto.
+        destruct H11 as [H11 | [H11 [H13 | H13]]]; auto.
+        right. split; auto. omega.
+    eapply mi_memval0 in Higns; eauto.
+
     destruct (Z_ge_dec ofs0 (ofs + Z_of_nat (length (encode_val chunk v1)))).
       apply setN_inj_outside; auto.
-      eapply mi_memval0 in H7; eauto.
-        rewrite encode_val_length in z. rewrite <- size_chunk_conv in z.
-        right. split; auto.
+      assert (notin_ignores ((b1, ofs, hi) :: igns) b1 ofs0) 
+        as Higns.
+        unfold notin_ignores.
+        inv H7.
+        constructor; auto.
+          destruct H11 as [H11 | [H11 [H13 | H13]]]; auto.
+          rewrite encode_val_length in z. rewrite <- size_chunk_conv in z.
+          contradict H13; omega.
+      eapply mi_memval0 in Higns; eauto.
 
       eapply setN_inj_inside; eauto. omega.
 
   destruct (zeq b3 b2). subst b3.
   (* block <> b1, block = b2 *)
-  rewrite setN_other. auto.
-  rewrite encode_val_length. rewrite <- size_chunk_conv. intros. 
-  assert (b2 <> b2).
-    eapply H1; eauto. 
+  unfold MoreMem.meminj_no_overlap in H1.
+  eapply H1 in n; eauto.
   congruence.
   (* block <> b1, block <> b2 *)
-  eauto.
+  eapply mi_memval0; eauto.
+    inv H7.
+    unfold notin_ignores.
+    constructor; auto.
 Qed.
 
-Lemma store_unmapped_inj:
-  forall b lo hi f chunk m1 b1 ofs v1 n1 m2,
-  mem_inj f b lo hi m1 m2 ->
+Lemma store_inside_inj2:
+  forall igns f m1 m2 chunk b1 b2 ofs v1 v2 n1 n2 delta hi,
+  mem_inj f ((b1,ofs,hi)::igns) m1 m2 ->
   store chunk m1 b1 ofs v1 = Some n1 ->
-  f b1 = None ->
-  mem_inj f b lo hi n1 m2.
+  MoreMem.meminj_no_overlap f ->
+  f b1 = Some (b2, delta) ->
+  MoreMem.val_inject f v1 v2 ->
+  store chunk m2 b2 (ofs+delta) v2 = Some n2 ->
+  mem_inj f ((b1,ofs+(size_chunk chunk),hi)::igns) n1 n2.
 Proof.
-  intros. inversion H.
-  constructor.
-(* access *)
-  eauto with mem.
-(* mem_contents *)
-  intros. 
-  rewrite (store_mem_contents _ _ _ _ _ _ H0).
-  rewrite update_o. eauto with mem. 
-  congruence.
+  intros.
+  eapply store_inside_inj2' in H; eauto.
+  destruct H as [n2' [J1 J2]].
+  uniq_result. auto.
 Qed.
 
-Lemma store_outside_inj:
-  forall b0 lo0 hi0 f m1 m2 chunk b ofs v m2',
-  mem_inj f b0 lo0 hi0 m1 m2 ->
+Lemma store_inside_inj_right:
+  forall igns f m1 m2 chunk b ofs v m2',
+  mem_inj f igns m1 m2 ->
   (forall b' delta ofs',
     f b' = Some(b, delta) ->
     perm m1 b' ofs' Nonempty ->
-    ofs' + delta < ofs \/ ofs' + delta >= ofs + size_chunk chunk) ->
+    in_ignores_with_size igns b' (ofs-delta) (size_chunk chunk)) ->
   store chunk m2 b ofs v = Some m2' ->
-  mem_inj f b0 lo0 hi0 m1 m2'.
+  mem_inj f igns m1 m2'.
 Proof.
   intros. inversion H. constructor.
 (* access *)
@@ -311,20 +508,23 @@ Proof.
 (* mem_contents *)
   intros. 
   rewrite (store_mem_contents _ _ _ _ _ _ H1).
-  unfold update. destruct (zeq b2 b). subst b2.
-  rewrite setN_outside. auto. 
+  unfold update. 
+  destruct (zeq b2 b); subst; auto.
+  rewrite setN_outside; auto. 
   rewrite encode_val_length. rewrite <- size_chunk_conv. 
-  eapply H0; eauto. 
-  eauto with mem.
+  eapply H0 in H3; eauto. 
+    eapply in_ignores_with_size__notin_ignores__inv in H3; eauto.
+      omega.
+      assert (J:=@size_chunk_pos chunk). omega.
 Qed.
 
 (** Preservation of allocations *)
 
 Lemma alloc_right_inj:
-  forall b9 lo9 hi9 f m1 m2 lo hi b2 m2',
-  mem_inj f b9 lo9 hi9 m1 m2 ->
+  forall igns f m1 m2 lo hi b2 m2',
+  mem_inj f igns m1 m2 ->
   alloc m2 lo hi = (m2', b2) ->
-  mem_inj f b9 lo9 hi9 m1 m2'.
+  mem_inj f igns m1 m2'.
 Proof.
   intros. injection H0. intros NEXT MEM.
   inversion H. constructor.
@@ -349,11 +549,11 @@ Local Transparent alloc.
 Qed.
 
 Lemma alloc_left_unmapped_inj:
-  forall b9 lo9 hi9 f m1 m2 lo hi m1' b1,
-  mem_inj f b9 lo9 hi9 m1 m2 ->
+  forall igns f m1 m2 lo hi m1' b1,
+  mem_inj f igns m1 m2 ->
   alloc m1 lo hi = (m1', b1) ->
   f b1 = None ->
-  mem_inj f b9 lo9 hi9 m1' m2.
+  mem_inj f igns m1' m2.
 Proof.
   intros. inversion H. constructor.
 (* access *)
@@ -370,13 +570,13 @@ Proof.
 Qed.
 
 Lemma free_right_inj:
-  forall b9 lo9 hi9 f m1 m2 b lo hi m2',
-  mem_inj f b9 lo9 hi9 m1 m2 ->
+  forall igns f m1 m2 b lo hi m2',
+  mem_inj f igns m1 m2 ->
   free m2 b lo hi = Some m2' ->
   (forall b1 delta ofs p,
     f b1 = Some(b, delta) -> perm m1 b1 ofs p ->
     lo <= ofs + delta < hi -> False) ->
-  mem_inj f b9 lo9 hi9 m1 m2'.
+  mem_inj f igns m1 m2'.
 Proof.
   intros. exploit free_result; eauto. intro FREE. inversion H. constructor.
 (* access *)
@@ -391,23 +591,23 @@ Proof.
   specialize (mi_memval0 _ _ _ _ H2 H3).
   assert (b=b2 /\ lo <= ofs+delta < hi \/ 
           (b<>b2 \/ ofs+delta<lo \/ hi <= ofs+delta)) as J 
-    by (unfold block; omega).
+    by (unfold Values.block; omega).
   destruct J as [[J1 J2] | J]; subst.
     specialize (H1 _ _ _ _ H2 H3). elimtype False; auto.
     rewrite (clearN_out _ _ _ _ _ _ J); auto.
 Qed.
 
 Lemma free_inj:
-  forall b9 lo9 hi9 f m1 m2 b1 b2 delta lo hi m1' m2',
+  forall igns f m1 m2 b1 b2 delta lo hi m1' m2',
   MoreMem.meminj_no_overlap f ->
   MoreMem.meminj_zero_delta f ->
-  mem_inj f b9 lo9 hi9 m1 m2 ->
+  mem_inj f igns m1 m2 ->
   free m1 b1 lo hi = Some m1' ->
   free m2 b2 (lo+delta) (hi+delta) = Some m2' ->
   f b1 = Some (b2, delta) ->
-  mem_inj f b9 lo9 hi9 m1' m2'.
+  mem_inj f igns m1' m2'.
 Proof.
-  intros b9 lo9 hi9 f m1 m2 b1 b2 delta lo hi m1' m2' J J' H H0 H1 H2.
+  intros igns f m1 m2 b1 b2 delta lo hi m1' m2' J J' H H0 H1 H2.
   exploit free_result; eauto. 
   intro FREE. inversion H. constructor.
 (* access *)
@@ -433,10 +633,10 @@ Proof.
   assert (FREE':=H0). apply free_result in FREE'.
   rewrite FREE'; simpl.   
   assert (b0=b1 /\ lo <= ofs < hi \/ (b1<>b0 \/ ofs<lo \/ hi <= ofs)) as J1
-    by (unfold block; omega).
+    by (unfold Values.block; omega).
   assert (b2=b3 /\ lo+delta <= ofs+delta < hi+delta \/ 
     (b2<>b3 \/ ofs+delta<lo+delta \/ hi+delta <= ofs+delta)) 
-    as J2 by (unfold block; omega).
+    as J2 by (unfold Values.block; omega).
   destruct J1 as [J1 | J1].
     destruct J1 as [J11 J12]; subst.
     eapply perm_free_2 with (p:=Nonempty) in H0; eauto.
@@ -460,10 +660,10 @@ Proof.
 Qed.
 
 Lemma free_left_nonmap_inj:
-  forall b9 lo9 hi9 f m1 m2 b lo hi m1' (Hprop: f b = None),
-  mem_inj f b9 lo9 hi9 m1 m2 ->
+  forall igns f m1 m2 b lo hi m1' (Hprop: f b = None),
+  mem_inj f igns m1 m2 ->
   Mem.free m1 b lo hi = Some m1' ->
-  mem_inj f b9 lo9 hi9 m1' m2.
+  mem_inj f igns m1' m2.
 Proof.
   intros. exploit Mem.free_result; eauto. intro FREE. inversion H. constructor.
 (* access *)
@@ -490,6 +690,329 @@ Lemma inject_id_zero_delta: MoreMem.meminj_zero_delta inject_id.
 Proof.
   unfold MoreMem.meminj_zero_delta, inject_id.
   intros. uniq_result. auto.
+Qed.
+
+Lemma notin_ignores_strengthen: forall b ofs igns2 igns1,
+  notin_ignores (igns1++igns2) b ofs ->
+  notin_ignores igns2 b ofs.
+Proof.
+  induction igns1 as [|[[]]]; simpl; intros; auto.
+    inv H. auto.
+Qed.
+
+Lemma mem_inj_ignores_weaken: forall mi igns' M1 M2 
+  (Hin : mem_inj mi igns' M1 M2) igns,
+  mem_inj mi (igns ++ igns') M1 M2.
+Proof.
+  induction igns; auto.
+    inv IHigns.  
+    constructor; auto.
+      intros.
+      simpl_env in H1.
+      apply mi_memval0; eauto using notin_ignores_strengthen.
+Qed.
+
+Lemma in_ignores_with_smaller_size: forall b ofs size1 size2 
+  (Hge: size1>=size2) igns,
+  in_ignores_with_size igns b ofs size1 ->
+  in_ignores_with_size igns b ofs size2.
+Proof.
+  unfold in_ignores_with_size.
+  intros.
+  destruct H as [b0 [lo0 [hi0 [H [J1 [J2 J3]]]]]]; subst.
+  exists b0. exists lo0. exists hi0.
+  split; auto. split; auto. split; omega.
+Qed.
+
+Lemma in_ignores_with_size_delta: forall b ofs delta size igns
+  (J:delta>=0),
+  in_ignores_with_size igns b ofs (delta+size) ->
+  in_ignores_with_size igns b (ofs+delta) size.
+Proof.
+  unfold in_ignores_with_size.
+  intros.
+  destruct H as [b0 [lo0 [hi0 [H [J1 [J2 J3]]]]]]; subst.
+  exists b0. exists lo0. exists hi0.
+  split; auto. split; auto. split; omega.
+Qed.
+
+Lemma mstore_aux_inside_inj_left: forall (TD : TargetData) (M2 : mem) 
+  (b : Values.block) igns (gv1 : GenericValue) (M1 : mem) (M1' : mem) ofs
+  (J2 : mstore_aux M1 gv1 b ofs = Some M1')
+  (Hin : mem_inj inject_id igns M1 M2)
+  (Higns: in_ignores_with_size igns b ofs (Z_of_nat (sizeGenericValue gv1))),
+  mem_inj inject_id igns M1' M2.
+Proof.
+  induction gv1 as [|[]]; simpl; intros.
+    uniq_result. auto.
+
+    inv_mbind.
+    rewrite inj_plus in Higns.
+    rewrite <- size_chunk_conv in Higns.
+    apply IHgv1 in H0; auto.
+      eapply store_inside_inj_left; eauto.
+        eapply in_ignores_with_smaller_size; eauto.
+          omega.
+      apply in_ignores_with_size_delta; auto.
+        assert (J:=@size_chunk_pos m). omega.
+Qed.
+
+Lemma mstore_aux_inside_inj_left': forall (TD : TargetData) (M2 : mem) 
+  (b : Values.block) lo hi
+  igns (gv1 : GenericValue) (M1 : mem) (M1' : mem) ofs
+  (J2 : mstore_aux M1 gv1 b ofs = Some M1')
+  (Hin : mem_inj inject_id igns M1 M2)
+  (Hrange: lo <= ofs /\ ofs + Z_of_nat (sizeGenericValue gv1) <= hi),
+  mem_inj inject_id ((b, lo, hi) :: igns) M1' M2.
+Proof.
+  intros.
+  simpl_env.
+  eapply mstore_aux_inside_inj_left; eauto.
+    apply mem_inj_ignores_weaken; auto.
+
+    unfold in_ignores_with_size.
+    exists b. exists lo. exists hi. simpl. 
+    split; auto. split; auto. omega.
+Qed.
+
+Lemma mstore_inside_inj_left: forall (TD : TargetData) (M1 : mem)
+  (gv1 : GenericValue) (a : align) (M1' : mem) t
+  (M2 : mem) igns (mb : mblock)
+  (H23 : mstore TD M1 ($ blk2GV TD mb # typ_pointer t $) t gv1 a = ret M1')
+  (Hin : mem_inj inject_id igns M1 M2),
+  mem_inj inject_id ((mb, 0, Size.to_Z (sizeGenericValue gv1))::igns) M1' M2.
+Proof.
+  intros.
+  apply mstore_inversion in H23.
+  rewrite Promotability.simpl_blk2GV in H23.
+  destruct H23 as [b [ofs [cm [J1 J2]]]].
+  inv J1.
+  rewrite Int.signed_repr in J2; auto using Promotability.min_le_zero_le_max.
+  eapply mstore_aux_inside_inj_left'; eauto.
+  unfold Size.to_Z.
+  split; omega.
+Qed.
+
+Lemma alloc_inject_id_inj:
+  forall igns m1 m2 lo hi b1 b2 m1' m2'
+  (Heq: nextblock m1 = nextblock m2)
+  (Hinj: mem_inj inject_id igns m1 m2)
+  (Hal1: alloc m1 lo hi = (m1', b1))
+  (Hal2: alloc m2 lo hi = (m2', b2)),
+  mem_inj inject_id igns m1' m2'.
+Proof.
+  intros. 
+  injection Hal1. intros NEXT1 MEM1; subst.
+  injection Hal2. intros NEXT2 MEM2; subst.
+  inversion Hinj. constructor.
+(* access *)
+  intros. unfold inject_id in H. inv H.
+  replace (ofs+0) with ofs by omega.
+  eapply valid_access_alloc_inv in H0; eauto.
+  destruct (eq_block b2 (nextblock m1)); subst.
+    apply valid_access_alloc_same with (chunk:=chunk)(ofs:=ofs) in Hal2; 
+      try solve [auto | omega | tauto].
+    rewrite Heq.
+    eapply valid_access_implies; try solve [eauto | constructor].
+
+    eapply valid_access_alloc_other in Hal2; eauto.
+    apply mi_access0 with (b2:=b2)(delta:=0) in H0; auto.
+    replace (ofs+0) with ofs in H0 by omega. auto.
+(* mem_contents *)
+  simpl.
+  intros. unfold inject_id in H. inv H.
+  eapply perm_alloc_inv in H0; eauto.
+  destruct (zeq b2 (nextblock m1)); subst.
+    rewrite <- Heq.
+    repeat rewrite update_s. constructor.
+
+    apply mi_memval0 with (b2:=b2)(delta:=0) in H0; auto.
+    repeat (rewrite update_o; try solve [auto | congruence]).
+Qed.
+
+Lemma notin_ignores_with_smaller_size: forall b ofs size1 size2 
+  (Hge: size1>=size2) igns,
+  notin_ignores_with_size igns b ofs size1 ->
+  notin_ignores_with_size igns b ofs size2.
+Proof.
+  unfold notin_ignores_with_size.
+  intros.
+  induction H; simpl; auto.
+    destruct x as [[b0 lo0] hi0].
+    constructor; auto.
+      destruct H as [H | [J1 [J2 | J3]]]; subst; auto.
+        right. split; auto. omega.
+Qed.
+
+Lemma mload_aux_inj2:
+  forall igns f b2 b1 (Hp1: MoreMem.meminj_no_overlap f)
+  (Hp2: MoreMem.meminj_zero_delta f)
+  mcs ofs delta gv1 gv2 m1 m2,
+  mem_inj f igns m1 m2 ->
+  mload_aux m1 mcs b1 ofs = Some gv1 ->
+  f b1 = Some (b2, delta) ->
+  notin_ignores_with_size igns b1 ofs (Z_of_nat (sizeMC mcs)) ->
+  mload_aux m2 mcs b2 (ofs + delta) = Some gv2 ->
+  gv_inject f gv1 gv2.
+Proof.
+  induction mcs; simpl; intros.
+    inv H0. inv H3. auto.
+
+    inv_mbind.
+    constructor.
+      eapply load_inj2; eauto.
+        eapply notin_ignores_with_smaller_size in H2; eauto.
+          rewrite inj_plus. rewrite <- size_chunk_conv. omega.
+      replace (ofs + delta + size_chunk a) with
+              (ofs + size_chunk a + delta) in HeqR0 by omega.
+      eapply IHmcs with (ofs:=ofs+size_chunk a); eauto.
+        rewrite inj_plus in H2. rewrite <- size_chunk_conv in H2. 
+        apply notin_ignores_with_size_delta; auto.
+          assert (J:=size_chunk_pos a). omega.
+Qed.
+
+Lemma mload_aux_inject_id_inj2:
+  forall igns b mcs ofs gv1 gv2 m1 m2,
+  mem_inj inject_id igns m1 m2 ->
+  mload_aux m1 mcs b ofs = Some gv1 ->
+  notin_ignores_with_size igns b ofs (Z_of_nat (sizeMC mcs)) ->
+  mload_aux m2 mcs b ofs = Some gv2 ->
+  gv1 = gv2.
+Proof.
+  intros.
+  replace ofs with (ofs+0) in H2 by omega.
+  eapply mload_aux_inj2 in H1; 
+    eauto using inject_id_no_overlap, inject_id_zero_delta.
+    apply gv_inject_id__eq in H1; auto.
+    unfold inject_id. auto.
+Qed.
+
+Lemma no_alias_with_blk__notin_ignores_with_size: forall b' ofs' m' size mbs
+  (Hnalias: 
+    Forall (fun re : Values.block * Z * Z =>
+            let '(mb, _, _) := re in
+            memory_props.MemProps.no_alias_with_blk 
+              ((Vptr b' ofs', m') :: nil) mb) mbs),
+  notin_ignores_with_size mbs b' (Int.signed 31 ofs') size.
+Proof.
+  unfold notin_ignores_with_size.
+  induction 1; simpl; auto.
+    destruct x as [[]]. simpl in H.
+    constructor; auto.
+Qed.
+
+Lemma mstore_aux_mapped_inj2: forall igns f b1 b2 delta
+  (Hp: MoreMem.meminj_no_overlap f)
+  (Hf: f b1 = Some (b2, delta)) gvs1 gvs2 m1 n1 m2 n2 ofs
+  (Hmsim: mem_inj f igns m1 m2) (Hst1: mstore_aux m1 gvs1 b1 ofs = Some n1)
+  (Hinj: gv_inject f gvs1 gvs2)
+  (Hst2: mstore_aux m2 gvs2 b2 (ofs + delta) = Some n2),
+  mem_inj f igns n1 n2.
+Proof.
+  induction gvs1 as [|[]]; simpl; intros.
+    inv Hst1. inv Hinj. inv Hst2. auto.
+
+    inv Hinj. simpl in Hst2.
+    inv_mbind.
+    assert (mem_inj f igns m3 m0) as Hinj'.
+      eapply store_mapped_inj2 in Hmsim; eauto.
+    replace (ofs + delta + size_chunk m) with
+            (ofs + size_chunk m + delta) in H0 by omega.
+    eapply IHgvs1; eauto.
+Qed.
+
+Lemma mstore_aux_inject_id_mapped_inj2: forall igns b gvs m1 n1 m2 n2 ofs
+  (Hmsim: mem_inj inject_id igns m1 m2) 
+  (Hst1: mstore_aux m1 gvs b ofs = Some n1)
+  (Hst2: mstore_aux m2 gvs b ofs = Some n2),
+  mem_inj inject_id igns n1 n2.
+Proof.
+  intros.
+  replace ofs with (ofs+0) in Hst2 by omega.
+  eapply mstore_aux_mapped_inj2 in Hmsim; 
+    eauto using inject_id_no_overlap, inject_id_zero_delta.
+    unfold inject_id. auto.
+    apply gv_inject_id__refl; auto.
+Qed.
+
+Lemma mstore_aux_store_inside_inj2': forall igns f b1 b2 delta
+  (Hp: MoreMem.meminj_no_overlap f)
+  (Hf: f b1 = Some (b2, delta)) hi gvs1 gvs2 m1 n1 m2 n2 ofs
+  (Hmsim: mem_inj f ((b1,ofs,hi)::igns) m1 m2) (Hst1: mstore_aux m1 gvs1 b1 ofs = Some n1)
+  (Hinj: gv_inject f gvs1 gvs2)
+  (Hst2: mstore_aux m2 gvs2 b2 (ofs + delta) = Some n2),
+  mem_inj f ((b1,ofs+Z_of_nat (sizeGenericValue gvs1),hi)::igns) n1 n2.
+Proof.
+  induction gvs1 as [|[]]; simpl; intros.
+    inv Hst1. inv Hinj. inv Hst2. 
+    replace (ofs+0) with ofs by omega.
+    auto.
+
+    inv Hinj. simpl in Hst2.
+    inv_mbind.
+    assert (mem_inj f ((b1,ofs+size_chunk m,hi)::igns) m3 m0) as Hinj'.
+      eapply store_inside_inj2 in Hmsim; eauto.
+    replace (ofs + delta + size_chunk m) with
+            (ofs + size_chunk m + delta) in H0 by omega.
+    rewrite inj_plus.
+    rewrite <- size_chunk_conv.
+    replace (ofs + (size_chunk m + Z_of_nat (sizeGenericValue gvs1))) with
+            (ofs + size_chunk m + Z_of_nat (sizeGenericValue gvs1)) by omega.
+    eapply IHgvs1; eauto.
+Qed.
+
+Lemma notin_ignores__add_empty: forall b hi b1 ofs igns
+  (Hnotin : notin_ignores igns b1 ofs),
+  notin_ignores ((b, hi, hi) :: igns) b1 ofs.
+Proof.
+  unfold notin_ignores.
+  intros.
+  constructor; auto. 
+    destruct (zeq b1 b); subst; auto.
+    right.
+    split; auto.
+      omega.
+Qed.
+
+Lemma mem_inj__remove_empty_igns: forall f b hi igns n1 n2
+  (Hmsim : mem_inj f ((b, hi, hi) :: igns) n1 n2),
+  mem_inj f igns n1 n2.
+Proof.
+  intros.
+  inv Hmsim.
+  constructor; auto.
+    intros.
+    apply mi_memval0; auto using notin_ignores__add_empty.
+Qed.
+
+Lemma mstore_aux_inside_inj2: forall igns f b1 b2 delta
+  (Hp: MoreMem.meminj_no_overlap f)
+  (Hf: f b1 = Some (b2, delta)) gvs1 gvs2 m1 n1 m2 n2 ofs
+  (Hmsim: mem_inj f ((b1,ofs,ofs+Z_of_nat (sizeGenericValue gvs1))::igns) m1 m2) 
+  (Hst1: mstore_aux m1 gvs1 b1 ofs = Some n1)
+  (Hinj: gv_inject f gvs1 gvs2)
+  (Hst2: mstore_aux m2 gvs2 b2 (ofs + delta) = Some n2),
+  mem_inj f igns n1 n2.
+Proof.
+  intros.
+  eapply mstore_aux_store_inside_inj2' in Hmsim; eauto.
+  eapply mem_inj__remove_empty_igns; eauto.
+Qed.
+
+Lemma mstore_aux_inject_id_inside_inj2: forall igns b
+  gvs m1 n1 m2 n2 ofs
+  (Hmsim: mem_inj inject_id 
+            ((b,ofs,ofs+Z_of_nat (sizeGenericValue gvs))::igns) m1 m2) 
+  (Hst1: mstore_aux m1 gvs b ofs = Some n1)
+  (Hst2: mstore_aux m2 gvs b ofs = Some n2),
+  mem_inj inject_id igns n1 n2.
+Proof.
+  intros.
+  replace ofs with (ofs+0) in Hst2 by omega.
+  eapply mstore_aux_inside_inj2 in Hmsim; 
+    eauto using inject_id_no_overlap, inject_id_zero_delta.
+    unfold inject_id. auto.
+    apply gv_inject_id__refl; auto.
 Qed.
 
 End SASmsim.
